# Fourier Representation

## Four repentations of Fourier
|           | Continuous | Discrete     |
| --------- | ---------- | ------------ |
| Periodic  | FS         | DTFS         |
| Aperiodic | FT         | DTFT<br><br> |

$$
\begin{align*}
y[n]&=\sum_{k=-\infty}^{\infty}h[k]x[n-k]\\
&=\sum_{k=-\infty}^{\infty}h[k]e^{j\Omega(n-k)}\\
&=\sum_{k=-\infty}^{\infty}h[k]e^{j\Omega n}e^{-j\Omega k}\\
&=e^{j\Omega n}\sum_{k=-\infty}^{\infty}h[k]e^{-j\Omega k}\\
\end{align*}
$$

> why it becomes 
> $$ \sum_{k=-\infty}^{\infty}h[k]x[n-k] $$
> instead of 
> $$ \sum_{k=-\infty}^{\infty}x[k]h[n-k] $$
> $h[n] * x[n] = x[n]*h[n]$
> And moving all $n$ out is quite benificial for the following calculation.

Then why ?

Convolution are painful to calculate, but it's easy to analyze in frequency domain.
Therefore, we need to convert convolution to multiplication.

$$ x[n] = \sum_k a_k e^{j\Omega_k n} \implies y[n]=\sum_k a_kH(e^{j\Omega_k})e^{j\Omega_k n}$$


> TODO


