# LTI 

## Impulse Response if LTI system

# State Variable Representation

# The Convolution Sum
We can express $x[n]$ as a sum of time-shifted impulses.

$$
x[n]=\sum_{k=-\infty}^{\infty}x[k]\delta[n-k]
$$
> Notice that $x[k]$ 

Let $y[n]$ be the output of the system $H$ when the input is $x[n]$.

$$
y[n]=H\{\sum_{k=-\infty}^{\infty}x[k]\delta[n-k]\}
$$

As we know its a LTI system, we can move $H$

$$
y[n]=\sum_{k=-\infty}^{\infty}x[k]H\{\delta[n-k]\}
$$

$H{\{\delta[n-k]\}}$ can be written as $h[k]$. called impulse response. Therefore 

$$
y[n]=\sum_{k=-\infty}^{\infty}h[k]x[n-k]
$$

Such 

$$ \sum_{k=-\infty}^{\infty}A[k]B[k]$$
called convolution of $A$ and $B$ and denoted as $A*B$
Therefore we can write $y[n]$ as 
$$h[n]*x[n]$$

## Convolution Sum Example
Consider   

$$y[n] = x[n] + x[n-1]$$
Then we can find $h[n]$ by following ideas

$$ \begin{align} 
x[n]&\rightarrow H \rightarrow y[n] \\
\delta[n] &\rightarrow H \rightarrow h[n]\\
\text{Let } x[n] &= \delta[n] \\
\text{Then } y[n] &= h[n] \\
\end{align} $$

So $h[n]=\delta[n]+\delta[n-1]$

$y[n]$ is a weighted sum of each time-shifted impulse response.
Let note 
$$y[n]=\sum_{k=-\infty}^{\infty}h[k]x[n-k]=\sum^\infty_{k=-\infty}w_n[k]$$
where $w_n[k]$ is the intermediate signal, useful when doing convolution.

### Example
Consider 

$$ h[k]=(\frac{3}{4})^ku[k]$$

If we want shifting or scaling, according to the precedence rule. We should first shift then scale. 

Let say we want shift left by n.

$$ h[k-n] = (\frac{3}{4})^{k+n}u[k+n]$$

Then we can scale it by -1.

$$ h[-k-n] = (\frac{3}{4})^{-k+n}u[-k+n]$$

#### Example
Consider 

$$ h[n]=\frac{1}{4}(u[n]-u[n-4])$$ 

![](attachs/Pasted%20image%2020240923173012.png)

$$x[n]=y[n]-u[n-10]$$
![](attachs/Pasted%20image%2020240923173033.png)

When convolution, one can separate into 3 parts.
![](attachs/Pasted%20image%2020240923175531.png)
![](attachs/Pasted%20image%2020240923175831.png)

#### Example
Consider 

$$y[n]-\rho y[n-1]=x[n]$$

let $x[n]=b^nu[n+4]$ and assume $b\neq\rho$ and system is causal.
Find $y[n]$
Then let $x[n]=\delta[n]$, $y[n]=h[n]$.
Therefore

$$ h[n]=\rho h[n-1]+\delta[n] $$ 

Since system is causal we can assume $h[n]=0$ for $n<0$.
Then we can find $h[n]$ by iteration.
$h[0]=1$, $h[1]=\rho$, $h[2]=\rho^2$, $h[3]=\rho^3$ ...
After that recall $y[n]=x[n]*h[n]$ which is
$$y[n]=\sum_{k=-\infty}^{\infty}x[k]h[n-k]$$

$$x[k]=\begin{cases}
b^k, -4\leq k \\
0, \text{otherwise} \\
\end{cases}$$

$$ h[n-k]=\begin{cases}
\rho^{n-k}, k\leq n \\
0, \text{otherwise} \\
\end{cases}$$

For $n<-4$, $x[n]*h[n]=0$., thus $y[n]=0$
For $n\geq-4$ $x[k]h[n-k]$

$$\begin{cases}
b^k\rho^{n-k}, -4\leq k\leq n \\
0, \text{otherwise} \\
\end{cases}$$

Then we convoluted it from $-4$ to $n$ to get $y[n]$.

$$\begin{align}
y[n]=&\sum_{k=-4}^{n}b^k\rho^{n-k}\\
=&\sum_{k=-4}^{n}b^k\rho^{n}\rho^{-k}\\
=\rho^n&\sum_{k=-4}^{n}(\frac{b}{\rho})^k\\
=\rho^n&\sum_{m=0}^{n+4}(\frac{b}{\rho})^{m-4}
; m = k + 4\\ 
=\rho^n&\sum_{m=0}^{n+4}(\frac{b}{\rho})^m(\frac{b}{\rho})^{-4}\\
=\rho^n(\frac{b}{\rho})^{-4}&\sum_{m=0}^{n+4}(\frac{b}{\rho})^m\\
\end{align}$$

Then we can solve the sum by using the formula of geometric series.

$$S=\frac{1-r^N}{1-r}$$

$$\begin{align}
y[n]=
&\rho^n(\frac{b}{\rho})^{-4}\frac{1-(\frac{b}{\rho})^{n+5}}{1-\frac{b}{\rho}}\\
=&\rho^n(\frac{b}{\rho})^{-4}\frac{p-(\frac{b^{n+5}}{\rho^{n+4}})}{p-b}\\
=&b^{-4}\frac{\rho^{n+5}-b^{n+5}}{\rho-b}\\
\end{align}$$

When $n \lt -4$, $y[n]=0$.

$$\begin{cases}
b^{-4}\frac{\rho^{n+5}-b^{n+5}}{\rho-b}, &n\geq-4 \\
0, &n\lt -4 \\
\end{cases}$$


